prototype and small update

coq/Main.v
@@ -1,11 +1,67 @@
 Require Import Autosubst.Autosubst.
+Require Import Coq.Program.Equality.
 
-Inductive term :=
-| Var (x : var)
-| App (e1 e2 : term)
-| Lam (e : {bind term}).
+(* ------- Syntax --------------- *)  
 
 Inductive type :=
 | Int
 | Top
-| Arr (A B : type).
+| Arr (A B : type).  
+
+Inductive term :=
+| Lit (n : nat)
+| Var (x : var)
+| Lam (e : {bind term})
+| App (e1 e2 : term)
+| Ann (e : term) (A : type).
+
+(* ------- Typing --------------- *)
+
+Inductive htype :=
+| HInt
+| HTop
+| HArr (A B : htype)
+| Hole (e : term).
+
+Fixpoint type_is_htype (A : type) :=
+  match A with
+  | Int => HInt
+  | Top => HTop
+  | Arr A B => HArr (type_is_htype A) (type_is_htype B)
+  end.
+
+Coercion type_is_htype : type >-> htype.
+
+Inductive ty (G : var -> type) : htype -> term -> type -> Prop :=
+| Ty_Lit  A n :
+  sub G Int A ->
+  ty G A (Lit n) Int
+| Ty_Var A B x :
+  G x = B -> sub G B A ->
+  ty G A (Var x) B
+| Ty_App e1 e2 A C D :
+  ty G (HArr (Hole e2) A) e1 (Arr C D) ->
+  ty G A (App e1 e2) D
+| Ty_Ann A (B : type) e :
+  ty G B e B -> sub G B A ->
+  ty G A (Ann e B) B
+| Ty_Lam1 e1 e A B B':
+  ty G Top e1 A ->
+  ty (A .: G) B' e B ->
+  ty G (HArr (Hole e1) B') (Lam e) (Arr A B)
+| Ty_Lam2 e A B' C :
+  ty (A .: G) B' e C ->
+  ty G (HArr A B') (Lam e) (Arr A C)
+with sub (G : var -> type) : htype -> htype -> Prop :=
+| S_Refl        : sub G HInt HInt
+| S_Top A       : sub G A HTop
+| S_Arr A B C D : sub G C A -> sub G B D -> sub G (HArr A B) (HArr C D)
+| S_Hole A A' e : ty G A e A' -> sub G (Hole e) A.
+
+Lemma ty_sub : forall A B e G,
+    ty G A e B ->
+    sub G B A.
+Proof.
+  intros. dependent induction H.
+Admitted.
+  
